noc/NOC.v
@@ -1,0 +1,206 @@
+Require Import Koika.Frontend.
+Require Import Koika.Std.
+Require Import Koika.Testing.
+Require Import noc.Router.
+
+Module Types.
+    Definition xy_cord :=
+    {|
+    struct_name := "xy_cord";
+    struct_fields :=
+      [
+        ("x" , bits_t 1);
+        ("y" , bits_t 1)
+      ]
+    |}.
+
+    Definition basic_flit :=
+    {|
+    struct_name := "basic_flit";
+    struct_fields :=
+      [
+        ("trg" , bits_t 2);
+        ("data" , bits_t 4)
+      ]
+    |}.
+
+End Types.
+
+Module Design.
+
+  Import Types.
+
+  Notation sz := 6.
+
+  Inductive reg_t :=
+      | r0_0d5_c
+      | r0_0d5_a
+      | r0d5_1_c
+      | r0d5_1_a
+      | r1_0d5_c
+      | r1_0d5_a
+      | r0d5_0_c
+      | r0d5_0_a
+      .
+
+
+Definition R reg :=
+  match reg with
+    | r0_0d5_c => bits_t (struct_sz basic_flit) 
+    | r0_0d5_a => bits_t (struct_sz basic_flit)
+    | r0d5_1_c => bits_t (struct_sz basic_flit)
+    | r0d5_1_a => bits_t (struct_sz basic_flit)
+    | r1_0d5_c => bits_t (struct_sz basic_flit)
+    | r1_0d5_a => bits_t (struct_sz basic_flit)
+    | r0d5_0_c => bits_t (struct_sz basic_flit)
+    | r0d5_0_a => bits_t (struct_sz basic_flit)
+  end.
+
+Definition r idx : R idx :=
+  match idx with
+    | r0_0d5_c => Bits.of_nat 6 49 
+    | r0_0d5_a => Bits.zero
+    | r0d5_1_c => Bits.zero
+    | r0d5_1_a => Bits.zero
+    | r1_0d5_c => Bits.zero
+    | r1_0d5_a => Bits.zero
+    | r0d5_0_c => Bits.zero
+    | r0d5_0_a => Bits.zero
+  end.
+
+Inductive rule_name_t :=
+  | route0_r
+  | route1_r
+  | route2_r
+  | route3_r.
+
+(* SEND FUNCTIONS*)
+Definition sendr0_0d5_a: UInternalFunction reg_t empty_ext_fn_t :=
+  {{ fun sendr0_0d5_a (value: bits_t 6) : unit_t =>
+    write0(r0_0d5_a, value)
+  }}.
+
+Definition sendr0_0d5_c: UInternalFunction reg_t empty_ext_fn_t :=
+  {{ fun sendr0_0d5_c (value: bits_t 6) : unit_t =>
+    write0(r0_0d5_c, value)
+  }}.
+
+Definition sendr0d5_1_a: UInternalFunction reg_t empty_ext_fn_t :=
+  {{ fun sendr0d5_1_a (value: bits_t 6) : unit_t =>
+    write0(r0d5_1_a, value)
+  }}.
+
+Definition sendr0d5_1_c: UInternalFunction reg_t empty_ext_fn_t :=
+  {{ fun sendr0d5_1_c (value: bits_t 6) : unit_t =>
+    write0(r0d5_1_c, value)
+  }}.
+
+Definition sendr1_0d5_a: UInternalFunction reg_t empty_ext_fn_t :=
+  {{ fun sendr1_0d5_a (value: bits_t 6) : unit_t =>
+    write0(r1_0d5_a, value)
+  }}.
+
+Definition sendr1_0d5_c: UInternalFunction reg_t empty_ext_fn_t :=
+  {{ fun sendr1_0d5_c (value: bits_t 6) : unit_t =>
+    write0(r1_0d5_c, value)
+  }}.
+
+Definition sendr0d5_0_a: UInternalFunction reg_t empty_ext_fn_t :=
+  {{ fun sendr0d5_0_a (value: bits_t 6) : unit_t =>
+    write0(r0d5_0_a, value)
+  }}.
+
+Definition sendr0d5_0_c: UInternalFunction reg_t empty_ext_fn_t :=
+  {{ fun sendr0d5_0_c (value: bits_t 6) : unit_t =>
+    write0(r0d5_0_c, value)
+  }}.
+
+(* RECIEVE FUNCTIONS*)
+Definition receiver0_0d5_a: UInternalFunction reg_t empty_ext_fn_t :=
+  {{ fun receiver0_0d5_a () : bits_t 6 =>
+    read0(r0_0d5_a)
+  }}.
+
+Definition receiver0_0d5_c: UInternalFunction reg_t empty_ext_fn_t :=
+  {{ fun receiver0_0d5_c () : bits_t 6 =>
+    read0(r0_0d5_c)
+  }}.
+
+Definition receiver0d5_1_a: UInternalFunction reg_t empty_ext_fn_t :=
+  {{ fun receiver0d5_1_a () : bits_t 6 =>
+    read0(r0d5_1_a)
+  }}.
+
+Definition receiver0d5_1_c: UInternalFunction reg_t empty_ext_fn_t :=
+  {{ fun receiver0d5_1_c () : bits_t 6 =>
+    read0(r0d5_1_c)
+  }}.
+
+Definition receiver1_0d5_a: UInternalFunction reg_t empty_ext_fn_t :=
+  {{ fun receiver1_0d5_a () : bits_t 6 =>
+     read0(r1_0d5_a)
+  }}.
+
+Definition receiver1_0d5_c: UInternalFunction reg_t empty_ext_fn_t :=
+  {{ fun receiver1_0d5_c () : bits_t 6 =>
+    read0(r1_0d5_c)
+  }}.
+
+Definition receiver0d5_0_a: UInternalFunction reg_t empty_ext_fn_t :=
+  {{ fun receiver0d5_0_a () : bits_t 6 =>
+    read0(r0d5_0_a)
+  }}.
+
+Definition receiver0d5_0_c: UInternalFunction reg_t empty_ext_fn_t :=
+  {{ fun receiver0d5_0_c () : bits_t 6 =>
+    read0(r0d5_0_c)
+  }}.
+
+
+Definition _routepr_r (r_addr: bits_t 2) (receive0 receive1 send0 send1: UInternalFunction reg_t empty_ext_fn_t) : uaction reg_t empty_ext_fn_t :=
+  {{
+      let r_addr := Ob~0~0 in
+      let m0 := receive0() ^ receive1() in
+       let addr := get(unpack(struct_t basic_flit, m0), trg) in
+    if addr[Ob~1] > r_addr[Ob~1] then
+        send0(m0)
+    else if addr[Ob~0] > r_addr[Ob~0] then
+        send1(m0)
+    else
+      pass
+  }}.
+
+
+
+(*Definition _routepr_r r send receive address : uaction r empty_ext_fn_t :=
+  {{
+      let newdata := receive  in
+      
+      if newdata then
+        let m0 := receive in
+        let addr0 := get(unpack(struct_t basic_flit, m0), trg) in
+        if !addr0 then
+          send(m0)
+        else
+          send(m0)
+      else
+        fail
+  }}. *)
+
+
+Inductive router_t :=
+  | rout4con r_addr
+  | rout6con 
+
+ Definition to_action rl :=
+    list 
+    end.
+
+
+  Definition schedule : scheduler :=
+  route0_r |> route1_r |> route3_r |>  route2_r |> done.
+
+  Definition rules :=
+    tc_rules R empty_Sigma to_action.
+
+End Design.
